providers/evercrypt/fst/EverCrypt.Hash.Incremental.fst
@@ -120,27 +120,36 @@ let create_in a r =
   assert (Hash.fresh_loc (Hash.footprint hash_state h2) h0 h2);
   assert (Hash.fresh_loc (B.loc_buffer buf) h0 h2);
   let s = State hash_state buf 0UL in
-  assert (Hash.fresh_loc (footprint s h2) h0 h2);
+  assert (Hash.fresh_loc (footprint_s h2 s) h0 h2);
+
+  let p = B.malloc r s 1ul in
+  let h20 = ST.get () in
+  assert (Hash.fresh_loc (B.loc_buffer p) h0 h20);
+  assert (B.(modifies loc_none h2 h20));
+  Hash.frame_invariant B.loc_none hash_state h2 h20;
+  Hash.frame_invariant_implies_footprint_preservation B.loc_none hash_state h2 h20;
+  assert (Hash.fresh_loc (footprint h20 p) h0 h20);
+  p
+
+let init a s =
+  let open LowStar.BufferOps in
+  let h1 = ST.get () in
+  let State hash_state buf _ = !*s in
 
   Hash.init #(G.hide a) hash_state;
-
-  let h3 = ST.get () in
-  Spec.Hash.Lemmas.update_multi_zero a (Hash.repr hash_state h3);
+  let h2 = ST.get () in
+  Spec.Hash.Lemmas.update_multi_zero a (Hash.repr hash_state h2);
   split_at_last_empty a;
-  assert (Hash.invariant hash_state h3);
-  assert (v 0ul <= B.length buf);
-  assert (
-    let blocks, rest = split_at_last a S.empty in
-    S.equal blocks S.empty /\ S.equal rest S.empty /\
-    Spec.Hash.(S.equal (update_multi a (init a) S.empty) (init a)));
-  assert (S.equal (Hash.repr hash_state h3) (Spec.Hash.init a));
+
+  s *= (State hash_state buf 0UL);
+  let h3 = ST.get () in
+  Hash.frame_invariant B.(loc_buffer s) hash_state h2 h3;
+  Hash.frame_invariant_implies_footprint_preservation B.(loc_buffer s) hash_state h2 h3;
+  assert (preserves_freeable s h1 h3);
+  assert (invariant h3 s);
   assert (hashes h3 s S.empty);
-  assert (freeable s h3);
-  assert (Hash.fresh_loc (footprint s h3) h0 h3);
-  assert (B.modifies (footprint s h3) h0 h3);
-  B.modifies_only_not_unused_in B.loc_none h0 h3;
-  assert (B.modifies B.loc_none h0 h3);
-  s
+  assert B.(modifies (footprint h1 s) h1 h3);
+  assert (equal_domains h1 h3)
 
 /// We keep the total length at run-time, on 64 bits, but require that it abides
 /// by the size requirements for the smaller hashes -- we're not interested at
@@ -148,37 +157,28 @@ let create_in a r =
 /// SHA384/512.
 
 inline_for_extraction noextract
-let rest a (total_len: UInt64.t): (x:UInt32.t { v x = v total_len % block_length a }) =
+let rest a (total_len: UInt64.t): (x:UInt32.t { U32.v x = U64.v total_len % block_length a }) =
   let open FStar.Int.Cast.Full in
-  uint64_to_uint32 (total_len % uint32_to_uint64 (Hacl.Hash.Definitions.block_len a))
+  uint64_to_uint32 (total_len `U64.rem` uint32_to_uint64 (Hacl.Hash.Definitions.block_len a))
 
 inline_for_extraction noextract
 let add_len (total_len: UInt64.t) (len: UInt32.t):
   Pure UInt64.t
-    (requires v total_len + v len < pow2 61)
-    (ensures fun x -> v x = v total_len + v len /\ v x < pow2 61)
+    (requires U64.v total_len + U32.v len < pow2 61)
+    (ensures fun x -> U64.v x = U64.v total_len + U32.v len /\ U64.v x < pow2 61)
 =
   assert_norm (pow2 61 < pow2 64);
-  total_len + Int.Cast.uint32_to_uint64 len
+  total_len `U64.add` Int.Cast.uint32_to_uint64 len
 
 #push-options "--z3rlimit 20"
 
 /// We split update into several versions, to all be simplified into a single
 /// large one at extraction-time.
 
+let total_len_h #a h (p: state a) =
+  State?.total_len (B.deref h p)
+
 /// Case 1: we just need to grow the buffer, no call to the hash function.
-val update_small:
-  a:Hash.alg ->
-  s:state a ->
-  prev:G.erased bytes ->
-  data: B.buffer UInt8.t ->
-  len: UInt32.t ->
-  Stack (state a)
-    (requires fun h0 ->
-      update_pre a s prev data len h0 /\
-      v len < block_length a - v (rest a (State?.total_len s)))
-    (ensures fun h0 s' h1 ->
-      update_post a s s' prev data len h0 h1)
 
 let split_at_last_small (a: Hash.alg) (b: bytes) (d: bytes): Lemma
   (requires (
@@ -251,33 +251,57 @@ let split_at_last_small (a: Hash.alg) (b: bytes) (d: bytes): Lemma
 #push-options "--z3rlimit 100"
 let add_len_small a (total_len: UInt64.t) (len: UInt32.t): Lemma
   (requires
-    v len < block_length a - v (rest a total_len) /\
-    v total_len + v len < pow2 61)
-  (ensures (rest a (add_len total_len len) = rest a total_len + len))
+    U32.v len < block_length a - U32.v (rest a total_len) /\
+    U64.v total_len + U32.v len < pow2 61)
+  (ensures (rest a (add_len total_len len) = rest a total_len `U32.add` len))
 =
-  FStar.Math.Lemmas.small_modulo_lemma_1 (v len) (block_length a);
-  FStar.Math.Lemmas.modulo_distributivity (v total_len) (v len) (block_length a)
+  FStar.Math.Lemmas.small_modulo_lemma_1 (U32.v len) (block_length a);
+  FStar.Math.Lemmas.modulo_distributivity (U64.v total_len) (U32.v len) (block_length a)
 #pop-options
 
-#push-options "--z3rlimit 100"
-let update_small a s prev data len =
+val update_small:
+  a:Hash.alg ->
+  s:state a ->
+  prev:G.erased bytes ->
+  data: B.buffer UInt8.t ->
+  len: UInt32.t ->
+  Stack unit
+    (requires fun h0 ->
+      update_pre a s prev data len h0 /\
+      U32.v len < block_length a - U32.v (rest a (total_len_h h0 s)))
+    (ensures fun h0 s' h1 ->
+      update_post a s prev data len h0 h1)
+
+#push-options "--z3rlimit 150"
+let update_small a p prev data len =
+  let open LowStar.BufferOps in
+  let s = !*p in
   let State hash_state buf total_len = s in
   let sz = rest a total_len in
   add_len_small a total_len len;
   let h0 = ST.get () in
   let buf1 = B.sub buf 0ul sz in
   let buf2 = B.sub buf sz len in
+
   B.blit data 0ul buf2 0ul len;
   let h1 = ST.get () in
   split_at_last_small a (G.reveal prev) (B.as_seq h0 data);
   Hash.frame_invariant (B.loc_buffer buf) hash_state h0 h1;
   Hash.frame_invariant_implies_footprint_preservation (B.loc_buffer buf) hash_state h0 h1;
-  let s' = State hash_state buf (add_len total_len len) in
-  assert (hashes h1 s' (S.append (G.reveal prev) (B.as_seq h0 data)));
-  assert (footprint s h0 == footprint s h1);
-  assert (preserves_freeable s h0 h1);
-  s'
+  assert (B.as_seq h1 data == B.as_seq h0 data);
+
+  p *= (State hash_state buf (add_len total_len len));
+  let h2 = ST.get () in
+  assert (B.as_seq h2 data == B.as_seq h1 data);
+  Hash.frame_invariant (B.loc_buffer p) hash_state h1 h2;
+  Hash.frame_invariant_implies_footprint_preservation (B.loc_buffer p) hash_state h1 h2;
+  assert (hashes h2 p (S.append (G.reveal prev) (B.as_seq h0 data)));
+  assert (footprint h0 p == footprint h2 p);
+  assert (preserves_freeable p h0 h2)
+
 #pop-options
+
+/// Case 2: we have no buffered data.
 
 #set-options "--z3rlimit 60"
 let split_at_last_blocks (a: Hash.alg) (b: bytes) (d: bytes): Lemma
@@ -348,22 +372,24 @@ let split_at_last_blocks (a: Hash.alg) (b: bytes) (d: bytes): Lemma
     blocks'';
   }
 
-/// Case 2: we have no buffered data.
+#push-options "--z3rlimit 150 --z3refresh"
 val update_empty_buf:
   a:Hash.alg ->
   s:state a ->
   prev:G.erased bytes ->
   data: B.buffer UInt8.t ->
   len: UInt32.t ->
-  Stack (state a)
+  Stack unit
     (requires fun h0 ->
       update_pre a s prev data len h0 /\
-      rest a (State?.total_len s) = 0ul)
+      rest a (total_len_h h0 s) = 0ul)
     (ensures fun h0 s' h1 ->
-      update_post a s s' prev data len h0 h1)
+      update_post a s prev data len h0 h1)
 
-#push-options "--z3rlimit 150"
-let update_empty_buf a s prev data len =
+// JP: this proof seems fragile -- diagnose?
+let update_empty_buf a p prev data len =
+  let open LowStar.BufferOps in
+  let s = !*p in
   let State hash_state buf total_len = s in
   let sz = rest a total_len in
   let h0 = ST.get () in
@@ -372,7 +398,7 @@ let update_empty_buf a s prev data len =
     S.equal blocks (G.reveal prev) /\
     S.equal rest S.empty);
   split_at_last_blocks a (G.reveal prev) (B.as_seq h0 data);
-  let n_blocks = len / Hacl.Hash.Definitions.block_len a in
+  let n_blocks = len `U32.div` Hacl.Hash.Definitions.block_len a in
   let data1_len = n_blocks `U32.mul` Hacl.Hash.Definitions.block_len a in
   let data2_len = len `U32.sub` data1_len in
   let data1 = B.sub data 0ul data1_len in
@@ -390,7 +416,11 @@ let update_empty_buf a s prev data len =
     (S.append (S.append (G.reveal prev) (B.as_seq h0 data1)) (B.as_seq h0 data2))
     (S.append (G.reveal prev) (S.append (B.as_seq h0 data1) (B.as_seq h0 data2))));
 
-  State hash_state buf (add_len total_len len)
+  p *= (State hash_state buf (add_len total_len len));
+  let h3 = ST.get () in
+  Hash.frame_invariant (B.loc_buffer p) hash_state h2 h3;
+  Hash.frame_invariant_implies_footprint_preservation (B.loc_buffer p) hash_state h2 h3;
+  ()
 #pop-options
 
 
@@ -402,15 +432,15 @@ val update_round:
   prev:G.erased bytes ->
   data: B.buffer UInt8.t ->
   len: UInt32.t ->
-  Stack (state a)
+  Stack unit
     (requires fun h0 ->
       update_pre a s prev data len h0 /\ (
-      let r = rest a (State?.total_len s) in
-      v len + v r = block_length a /\
+      let r = rest a (total_len_h h0 s) in
+      U32.v len + U32.v r = block_length a /\
       r <> 0ul))
-    (ensures fun h0 s' h1 ->
-      update_post a s s' prev data len h0 h1 /\
-      v (State?.total_len s') % block_length a = 0)
+    (ensures fun h0 _ h1 ->
+      update_post a s prev data len h0 h1 /\
+      U64.v (total_len_h h1 s) % block_length a = 0)
 
 let split_at_last_block (a: Hash.alg) (b: bytes) (d: bytes): Lemma
   (requires (
@@ -423,11 +453,13 @@ let split_at_last_block (a: Hash.alg) (b: bytes) (d: bytes): Lemma
 =
    ()
 
-let update_round a s prev data len =
+let update_round a p prev data len =
+  let open LowStar.BufferOps in
+  let s = !*p in
   let State hash_state buf_ total_len = s in
   let h0 = ST.get () in
   let sz = rest a total_len in
-  let diff = Hacl.Hash.Definitions.block_len a - sz in
+  let diff = Hacl.Hash.Definitions.block_len a `U32.sub` sz in
   let buf0 = B.sub buf_ 0ul (Hacl.Hash.Definitions.block_len a) in
   let buf1 = B.sub buf0 0ul sz in
   let buf2 = B.sub buf0 sz diff in
@@ -475,43 +507,45 @@ let update_round a s prev data len =
       Hash.invariant hash_state h2);
     ()
   );
-  let s' = State hash_state buf_ (add_len total_len len) in
-  assert (hashes h2 s' (S.append (G.reveal prev) (B.as_seq h0 data)));
-  s'
+  p *= (State hash_state buf_ (add_len total_len len));
+  let h3 = ST.get () in
+  Hash.frame_invariant (B.loc_buffer p) hash_state h2 h3;
+  Hash.frame_invariant_implies_footprint_preservation (B.loc_buffer p) hash_state h2 h3;
+  assert (hashes h3 p (S.append (G.reveal prev) (B.as_seq h0 data)))
 #pop-options
 
 #push-options "--z3rlimit 200"
-let update a s prev data len =
+let update a p prev data len =
+  let open LowStar.BufferOps in
+  let s = !*p in
   let State hash_state buf_ total_len = s in
   let sz = rest a total_len in
-  if len < Hacl.Hash.Definitions.block_len a - sz then
-    update_small a s prev data len
+  if len `U32.lt` (Hacl.Hash.Definitions.block_len a `U32.sub` sz) then
+    update_small a p prev data len
   else if sz = 0ul then
-    update_empty_buf a s prev data len
+    update_empty_buf a p prev data len
   else begin
     let h0 = ST.get () in
-    let diff = Hacl.Hash.Definitions.block_len a - sz in
+    let diff = Hacl.Hash.Definitions.block_len a `U32.sub` sz in
     let data1 = B.sub data 0ul diff in
-    let data2 = B.sub data diff (len - diff) in
-    let s1 = update_round a s prev data1 diff in
+    let data2 = B.sub data diff (len `U32.sub` diff) in
+    update_round a p prev data1 diff;
     let h1 = ST.get () in
-    let s2 = update_empty_buf a s1
-      (G.hide (S.append (G.reveal prev) (B.as_seq h0 data1))) data2 (len - diff)
-    in
+    update_empty_buf a p
+      (G.hide (S.append (G.reveal prev) (B.as_seq h0 data1))) data2 (len `U32.sub` diff);
     let h2 = ST.get () in
     (
       let prev = G.reveal prev in
-      assert (hashes h1 s1 (S.append prev (B.as_seq h0 data1)));
-      assert (hashes h2 s2 (S.append (S.append prev (B.as_seq h0 data1)) (B.as_seq h0 data2)));
+      assert (hashes h1 p (S.append prev (B.as_seq h0 data1)));
+      assert (hashes h2 p (S.append (S.append prev (B.as_seq h0 data1)) (B.as_seq h0 data2)));
       S.append_assoc prev (B.as_seq h0 data1) (B.as_seq h0 data2);
       assert (S.equal (S.append (B.as_seq h0 data1) (B.as_seq h0 data2)) (B.as_seq h0 data));
       assert (S.equal
         (S.append (S.append prev (B.as_seq h0 data1)) (B.as_seq h0 data2))
         (S.append prev (B.as_seq h0 data)));
-      assert (hashes h2 s2 (S.append prev (B.as_seq h0 data)));
+      assert (hashes h2 p (S.append prev (B.as_seq h0 data)));
       ()
-    );
-    s2
+    )
   end
 #pop-options
 
@@ -520,8 +554,10 @@ val mk_finish: a:Hash.alg -> finish_st a
 
 #reset-options "--z3rlimit 30 --max_fuel 0 --max_ifuel 0"
 inline_for_extraction noextract
-let mk_finish a s prev dst =
+let mk_finish a p prev dst =
+  let open LowStar.BufferOps in
   let h0 = ST.get () in
+  let s = !*p in
   let State hash_state buf_ total_len = s in
 
   push_frame ();
@@ -531,11 +567,11 @@ let mk_finish a s prev dst =
   assert (Hash.invariant hash_state h1);
 
   assert_norm (pow2 61 < pow2 125);
-  assert (v total_len < max_input_length a);
+  assert (U64.v total_len < max_input_length a);
   let buf_ = B.sub buf_ 0ul (rest a total_len) in
   assert (
     let r = rest a total_len in
-    (v total_len - v r) % block_length a = 0);
+    (U64.v total_len - U32.v r) % block_length a = 0);
 
   let tmp_hash_state = Hash.alloca a in
 
@@ -581,7 +617,7 @@ let mk_finish a s prev dst =
       finish a (
         update_multi a (Hash.repr tmp_hash_state h3)
           (S.append
-            (S.slice (B.as_seq h3 buf_) 0 (v (rest a total_len)))
+            (S.slice (B.as_seq h3 buf_) 0 (U32.v (rest a total_len)))
             (pad a (UInt64.v total_len))));
     (S.equal) { }
       finish a (
@@ -611,7 +647,7 @@ let mk_finish a s prev dst =
   Hash.frame_invariant B.(loc_region_only false (HS.get_tip h5)) hash_state h5 h6;
   Hash.frame_invariant_implies_footprint_preservation
     B.(loc_region_only false (HS.get_tip h5)) hash_state h5 h6;
-  assert (hashes h6 s (G.reveal prev));
+  assert (hashes h6 p (G.reveal prev));
 
   (*
    * AR: 02/14: This is hard. In emacs, the lemma calls are not needed
@@ -622,7 +658,7 @@ let mk_finish a s prev dst =
    *            -- The name of one non total arrow symbol (_288 vs _327)
    *            Can't do much about it, may be can investigate the gensym difference
    *)
-  let mloc = B.loc_union (B.loc_buffer dst) (footprint s h0) in
+  let mloc = B.loc_union (B.loc_buffer dst) (footprint h0 p) in
   B.modifies_remove_fresh_frame h0 h1 h6 mloc;
   B.popped_modifies h5 h6;
   assert (B.(modifies mloc h0 h6))
@@ -648,6 +684,7 @@ let finish a s prev dst =
   | SHA2_512 -> finish_sha512 s prev dst
 
 let free a s =
-  let State hash_state buf _ = s in
+  let open LowStar.BufferOps in
+  let State hash_state buf _ = !*s in
   Hash.free #(Ghost.hide a) hash_state;
   B.free buf
